Implement HKDF, build system, directory structure
This is the Dafny implementation of the HKDF as described in (https://tools.ietf.org/html/rfc5869), based on an initial version by Rustan Leino. The HKDF relies on an HMAC provided by a library. `CryptoMac.dfy` contains extern methods that are implemented in `hkdf-extern.cs` as wrappers around BouncyCastle. Supports SHA256 and SHA384 hash functions.

To make it testable I created a different directory structure and set up a lit configuration. The tests currently added are the HKDF test vectors as in github.com/aws/aws-encryption-sdk-c.
The negative test case (test vector 6), when no hash algorithm is chosen, is not yet implemented.

src/HKDF-extern.cs
@@ -1,0 +1,84 @@
+using System;
+using System.Numerics;
+
+public static class Util {
+  public static int BigIntegerToInt(BigInteger x) {
+    try {
+      return (int) x;
+    } catch(OverflowException e) {
+      // TODO: error handling
+      Console.WriteLine(e.ToString());
+      throw e;
+    }
+  }
+}
+
+namespace Arrays {
+  public partial class Array {
+    public static void copy<T>(T[] source, BigInteger length, out T[] dest) {
+      dest = new T[Util.BigIntegerToInt(length)];
+      System.Array.Copy(source, dest, Util.BigIntegerToInt(length));
+    }
+    public static void copyTo<T>(T[] source, T[] dest, BigInteger offset) {
+      source.CopyTo(dest, Util.BigIntegerToInt(offset)); 
+    }
+  }
+}
+
+
+namespace BouncyCastleCryptoMac {
+
+  using Org.BouncyCastle.Crypto;
+  public partial class HMac {
+
+    private Org.BouncyCastle.Crypto.Macs.HMac bcHMac;
+
+    public HMac(Digests.HMAC_ALGORITHM algorithm) {
+      IDigest digest;
+      if(algorithm.is_HmacSHA256) {
+        digest = new Org.BouncyCastle.Crypto.Digests.Sha256Digest();
+        bcHMac = new Org.BouncyCastle.Crypto.Macs.HMac(digest);
+      }
+      if(algorithm.is_HmacSHA384) {
+        digest = new Org.BouncyCastle.Crypto.Digests.Sha384Digest();
+        bcHMac = new Org.BouncyCastle.Crypto.Macs.HMac(digest);
+      }
+    }
+
+    public Dafny.Sequence<char> getAlgorithmName() {
+      return Dafny.Sequence<char>.FromString(bcHMac.AlgorithmName);
+    }
+
+    public BigInteger getMacSize() {
+      return new BigInteger(bcHMac.GetMacSize());
+    }
+    
+    public void init(CipherParameters ps) {
+      if(ps.is_KeyParameter) {
+        var bcKeyParameter = new Org.BouncyCastle.Crypto.Parameters.KeyParameter(ps.key);
+        bcHMac.Init(bcKeyParameter);
+      }
+    }
+
+    public void reset() {
+      bcHMac.Reset();
+    }
+ 
+    public void updateSingle(byte input) {
+      bcHMac.Update(input);
+    }
+ 
+    public void update(byte[] input , BigInteger inOff, BigInteger len) {
+      bcHMac.BlockUpdate(input, Util.BigIntegerToInt(inOff), Util.BigIntegerToInt(len));
+    }
+ 
+    public void doFinal(byte[] output, BigInteger outOff, out BigInteger retVal) {
+      retVal = new BigInteger(bcHMac.DoFinal(output, Util.BigIntegerToInt(outOff)));
+    }
+
+    public Org.BouncyCastle.Crypto.IDigest getUnderlyingDigest() {
+      return bcHMac.GetUnderlyingDigest();
+    }
+
+  }
+}
