src/StandardLibrary.dfy
@@ -1,7 +1,14 @@
+// =============== Basic library stuff ===============
+
 module StandardLibrary {
+  export
+    reveals byte, WrapIntoByte, Option, Integer_Upper_Bound
+    provides MulLemma, Fill, SeqPrefixLemma, SplitArray
+ 
   datatype Option<T> = None | Some(get: T)
 
   newtype byte = x | 0 <= x < 256
+
   newtype int32 = x | -0x8000_0000 <= x < 0x8000_0000
 
   newtype uint64 = x | 0 <= x < 0x1_0000_0000_0000_0000
@@ -15,5 +22,40 @@ module StandardLibrary {
     forall i | 0 <= i < |s| {
       a[i] := (s[i] as int % 256) as byte;
     }
+  }
+
+  function method WrapIntoByte(y: int): byte
+    requires 0 <= y < 256
+  {
+    y as byte
+  }
+ 
+  // The Java library defines Integer.MAX_VALUE as 0x7fff_ffff.
+  const Integer_Upper_Bound := 0x8000_0000
+
+  // multiplication with a non-negative number is monotonic
+  lemma MulLemma(a: int, b: int, n: nat)
+    requires a <= b
+    ensures a*n <= b*n
+  {
+  }
+ 
+  function Fill<T>(value: T, n: nat): seq<T>
+    ensures |Fill(value, n)| == n
+    ensures forall i :: 0 <= i < n ==> Fill(value, n)[i] == value
+  {
+    if n > 0 then [value] + Fill(value, n-1) else []
+  }
+ 
+  lemma SeqPrefixLemma<T>(a: seq<T>, b: seq<T>, n: nat)
+    requires n <= |a| && a <= b
+    ensures a[..n] == b[..n]
+  {
+  }
+ 
+  lemma SplitArray<T>(a: array<T>, m: nat, n: nat)
+    requires m + n <= a.Length
+    ensures a[..m+n] == a[..m] + a[m..m+n]
+  {
   }
 }
