src/CryptoLibrary.dfy
@@ -1,0 +1,69 @@
+// =============== Crypto library stuff ===============
+include "StandardLibrary.dfy"
+
+module {:extern "Digests"} Digests {
+  datatype {:extern "HMAC_ALGORITHM"} HMAC_ALGORITHM = HmacSHA256  | HmacSHA384 | HmacNOSHA
+}
+
+module HKDFSpec {
+  import opened StandardLibrary
+  import opened Digests
+  
+  // Hash length in octets, e.g. HashLength(SHA256) = 256 = 32 * 8
+  function {:axiom} HashLength(algorithm: HMAC_ALGORITHM): nat
+    ensures algorithm == HmacSHA256 ==> HashLength(algorithm) == 32
+    ensures algorithm == HmacSHA384 ==> HashLength(algorithm) == 48
+
+  function {:axiom} Hash(algorithm: HMAC_ALGORITHM, key: seq<byte>, message: seq<byte>): seq<byte>
+    ensures |Hash(algorithm, key, message)| == HashLength(algorithm)
+
+  // return T(i)
+  function HashIterate(algorithm: HMAC_ALGORITHM, key: seq<byte>, info: seq<byte>, i: nat): seq<byte>
+    requires 0 <= i < 256
+    decreases i, 1
+  {
+    if i == 0 then [] else
+    Hash(algorithm, key, HashIterateMsg(algorithm, key, info, i))
+  }
+
+  // return T(i-1) | info | i
+  function HashIterateMsg(algorithm: HMAC_ALGORITHM, key: seq<byte>, info: seq<byte>, i: nat): seq<byte>
+    requires 1 <= i < 256
+    decreases i, 0
+  {
+    HashIterate(algorithm, key, info, i-1) + info + [WrapIntoByte(i)]
+  }
+ 
+  // return T(1) | T(2) | ... | T(n)
+  function AccumulatedHashIterates(algorithm: HMAC_ALGORITHM, key: seq<byte>, info: seq<byte>, n: nat): seq<byte>
+    requires 0 <= n < 256
+    decreases n
+  {
+    if n == 0 then [] else
+      AccumulatedHashIterates(algorithm, key, info, n-1) + HashIterate(algorithm, key, info, n)
+  }
+ 
+  lemma AccHashIterLength(algorithm: HMAC_ALGORITHM, key: seq<byte>, info: seq<byte>, n: nat)
+    requires 0 <= n < 256
+    ensures |AccumulatedHashIterates(algorithm, key, info, n)| == n * HashLength(algorithm)
+  {
+  }
+ 
+  lemma AccHashIterPrefix(algorithm: HMAC_ALGORITHM, key: seq<byte>, info: seq<byte>, m: nat, n: nat)
+    requires 0 <= m <= n < 256
+    ensures AccumulatedHashIterates(algorithm, key, info, m) <= AccumulatedHashIterates(algorithm, key, info, n)
+  {
+    if m == n {
+    } else {
+      AccHashIterPrefix(algorithm, key, info, m, n-1);
+    }
+  }
+ 
+  function IteratedHash(algorithm: HMAC_ALGORITHM, key: seq<byte>, info: seq<byte>): (result: seq<byte>)
+    ensures |result| == 255 * HashLength(algorithm)
+  {
+    AccHashIterLength(algorithm, key, info, 255);
+    AccumulatedHashIterates(algorithm, key, info, 255)
+  }
+ 
+}
