src/HKDF.dfy
@@ -1,0 +1,139 @@
+/* HmacSha256Kdf.dfy
+* Rustan Leino, 28 Dec 2017.
+* Matthias Schlaipfer, 11 June 2019
+* This is a transcription of David Cok's HmacSha256Kdf.java into Dafny.
+* There are three major parts:
+*   0. Basic library stuff
+*      Routine definitions and specifications. (Feel free to skip reading this part.)
+*   1. Crypto library stuff
+*      Formalizes the Extract-and-Expand HKDF specifications and models the Mac class
+*      in the Java library.
+*   2. The code to be verified
+*      The hkdf routine and its correctness proof.
+*
+* "nfv" stands for necessary for verification
+*/
+ 
+include "StandardLibrary.dfy"
+include "Arrays.dfy"
+include "CryptoLibrary.dfy" 
+include "CryptoMac.dfy"
+ 
+// =============== The code to be verified ===============
+ 
+/**
+  * Implementation of the https://tools.ietf.org/html/rfc5869 hmac based key derivation function
+  */
+module HKDF {
+  import opened StandardLibrary
+  import opened Arrays
+  import opened Digests
+  import opened HKDFSpec
+  import opened BouncyCastleCryptoMac
+ 
+  method hkdf_Extract(which_sha: HMAC_ALGORITHM, hmac: HMac, salt: array<byte>, ikm: array<byte>) returns (prk: array<byte>)
+    requires hmac.algorithm == which_sha && salt.Length != 0
+    modifies hmac
+    ensures prk[..] == Hash(which_sha, salt[..], ikm[..])
+  {
+    var params: CipherParameters := KeyParameter(salt);
+    hmac.init(params);
+    assert hmac.InputSoFar + ikm[..] == ikm[..]; // nfv
+    hmac.updateAll(ikm);
+    prk := new byte[hmac.getMacSize()];
+    var _ := hmac.doFinal(prk, 0);
+    return prk;
+  }
+
+  method hkdf_Expand(which_sha: HMAC_ALGORITHM, hmac: HMac, prk: array<byte>, info: array<byte>, n: int) returns (a: array<byte>)
+    requires hmac.algorithm == which_sha && 1 <= n <= 255 && prk.Length != 0
+    requires info.Length + hmac.getMacSize() + 1 < Integer_Upper_Bound
+    modifies hmac
+    ensures fresh(a)
+    ensures a[..] == AccumulatedHashIterates(which_sha, prk[..], info[..], n)
+    ensures a.Length == n * hmac.getMacSize();
+  {
+    var params: CipherParameters := KeyParameter(prk);
+    hmac.init(params);
+    ghost var gKey := hmac.initialized.get;
+
+    ghost var s: seq<byte> := [];  // s == T(0)
+    a := new byte[n * hmac.getMacSize()];
+    var Ti: array<byte> := new byte[hmac.getMacSize()];
+
+    // T(1)
+    hmac.updateAll(info);
+    hmac.updateSingle(WrapIntoByte(1));
+    var _ := hmac.doFinal(Ti, 0);
+    Array.copyTo(Ti, a, 0);
+    s := s + Ti[..];
+
+    var i := 1;
+    while i < n
+      invariant 1 <= i <= n
+      invariant Ti.Length == HashLength(which_sha)
+      invariant Ti[..] == HashIterate(which_sha, prk[..], info[..], i)[..]
+      invariant s == AccumulatedHashIterates(which_sha, prk[..], info[..], i)     // s == T(1) | ... | T(i)
+      invariant s == a[..i * hmac.getMacSize()]
+      invariant hmac.initialized.Some? && hmac.initialized.get == gKey
+      invariant hmac.InputSoFar == []
+    {
+      // T(i+1)
+      hmac.updateAll(Ti);
+      hmac.updateAll(info);
+      hmac.updateSingle(WrapIntoByte(i+1));
+      assert hmac.InputSoFar[..] == Ti[..] + info[..] + [WrapIntoByte(i+1)]; // nfv
+      var _ := hmac.doFinal(Ti, 0);
+      Array.copyTo(Ti, a, i*hmac.getMacSize());
+      s := s + Ti[..]; // s == T(1) | ... | T(i) | T(i+1)
+      i := i + 1;
+    }
+  }
+
+  /**
+   * The RFC 5869 KDF. Outputs L bytes of output key material.
+   **/
+  method hkdf(which_sha: HMAC_ALGORITHM, salt: array<byte>, ikm: array<byte>, info: array<byte>, L: int) returns (okm: array<byte>)
+    requires which_sha == HmacSHA256 || which_sha == HmacSHA384
+    requires 0 <= L <= 255 * HashLength(which_sha)
+    requires info.Length + HashLength(which_sha) + 1 < Integer_Upper_Bound
+    ensures fresh(okm)
+    ensures okm.Length == L
+    ensures
+      // Extract:
+      var prk := Hash(which_sha, if salt.Length==0 then Fill(0, HashLength(which_sha)) else salt[..], ikm[..]);
+      // Expand:
+      okm[..L] == IteratedHash(which_sha, prk, info[..])[..L]
+  {
+    if L == 0 {
+      return new byte[0];
+    }
+    var hmac := new HMac(which_sha);
+ 
+    var mysalt: array<byte>;
+    if salt.Length != 0 { 
+      mysalt := salt; 
+    } else { 
+      mysalt := new byte[hmac.getMacSize()](_ => 0); 
+    }
+    assert mysalt[..] == if salt.Length==0 then Fill(0, hmac.getMacSize()) else salt[..]; // nfv
+ 
+    var n := 1 + (L-1) / hmac.getMacSize();  // note, since L and HMAC_SIZE are strictly positive, this gives the same result in Java as in Dafny
+    assert n * hmac.getMacSize() >= L;
+    var prk := hkdf_Extract(which_sha, hmac, mysalt, ikm);
+
+    okm := hkdf_Expand(which_sha, hmac, prk, info, n);
+
+    // if necessary, trim padding
+    if okm.Length > L {
+      okm := Array.copy(okm, L);
+    }
+    calc {
+      okm[..L];
+    ==
+      AccumulatedHashIterates(which_sha, prk[..], info[..], n)[..L];
+    ==  { AccHashIterPrefix(which_sha, prk[..], info[..], n, 255); }
+      IteratedHash(which_sha, prk[..], info[..])[..L];
+    }
+  }
+}
