Makefile
@@ -1,0 +1,79 @@
+ifeq ($(OS),Windows_NT)
+  DAFNY = Dafny.exe
+else
+  DAFNY = dafny
+endif
+SRCDIR   = src
+BUILDDIR = build
+
+# Copied from previous one
+_SRC = \
+  StandardLibrary.dfy \
+	ByteOrder.dfy \
+	AwsCrypto.dfy \
+	ByteBuf.dfy \
+	KeyringTrace.dfy \
+	EDK.dfy \
+	Cipher.dfy \
+	Frame.dfy \
+	Materials.dfy \
+	DefaultCMM.dfy \
+	Session.dfy
+SRC  = $(patsubst %,$(SRCDIR)/%,$(_SRC))
+SRCV = $(patsubst %, %.verified, $(SRC))
+
+DEPS     = src/HKDF-extern.cs\
+			lib/BouncyCastle.1.8.5/lib/BouncyCastle.Crypto.dll
+
+DLL      = HKDF.dll
+_OBJ     = $(DLL) HKDF.cs HKDF.pdb
+OBJ      = $(patsubst %,$(BUILDDIR)/%,$(_OBJ))
+
+DPARAMS  = /out:$(BUILDDIR)/HKDF
+
+SRCOBJ   = $(patsubst %,$(SRCDIR)/%,$(_OBJ))
+
+.PHONY: clean deps all hkdf test help lit
+
+all: hkdf
+
+# Verify each file separately
+$(SRCDIR)/%.dfy.verified: $(SRCDIR)/%.dfy
+	$(DAFNY) $^ /compile:0 && touch $@
+
+_HKDFSRC = HKDF.dfy StandardLibrary.dfy Arrays.dfy CryptoLibrary.dfy CryptoMac.dfy
+HKDFSRC  = $(patsubst %,$(SRCDIR)/%,$(_HKDFSRC))
+HKDFSRCV = $(patsubst %, %.verified, $(HKDFSRC))
+
+# Compile output without verification, we already have verified each file
+$(OBJ): $(HKDFSRCV) $(SRCDIR)/HKDF-extern.cs $(DEPS)
+	$(DAFNY) $(DPARAMS) $(HKDFSRC) $(DEPS) /compile:2 /noVerify /noIncludes
+
+hkdf: deps $(BUILDDIR)/$(DLL)
+
+lib/BouncyCastle.1.8.5/lib/BouncyCastle.Crypto.dll:
+	nuget install
+
+lit:
+	pip install lit
+
+test: 
+	lit test
+
+deps: lib/BouncyCastle.1.8.5/lib/BouncyCastle.Crypto.dll lit
+
+# Copied from previous one
+run: EncryptDecryptString.exe
+	mono EncryptDecryptString.exe
+
+# Copied from previous one
+EncryptDecryptString.exe: $(SOURCES)
+	$(DAFNY) $(DPARAMS)/"$@" $^
+
+clean:
+	rm $(BUILDDIR)/*
+	rm $(SRCV)
+	rm -rf lib/*
+
+help:
+	@echo "Usage: make {all, hkdf, deps, lit, clean, help}"
