README.md
@@ -1,7 +1,17 @@
-## AWS Encryption SDK Dafny
+# AWS Encryption SDK Dafny
+
+![Build Status - master branch](https://codebuild.us-west-2.amazonaws.com/badges?uuid=eyJlbmNyeXB0ZWREYXRhIjoiVmIzeGwwQmY5bXdMQXg2aVBneWtDc3FHSWRHTjYrNnVUem9nNXJFUmY2Rk1yRnJvSjJvK3JCL2RScFRjSVF1UjA1elR3L0xpTVpiNmRZS0RyWjJpTnBFPSIsIml2UGFyYW1ldGVyU3BlYyI6InBBQm1tT1BPNjB3RU9XUS8iLCJtYXRlcmlhbFNldFNlcmlhbCI6MX0%3D&branch=master)
 
 AWS Encryption SDK for Dafny
 
 ## License
 
 This library is licensed under the Apache 2.0 License. 
+
+## Building (the HKDF)
+
+* You need to have a working Dafny installation and have Dafny.exe on your path
+  * Dafny itself depends on Boogie and an SMT solver such as Z3.
+* Download the BouncyCastle DLL by running e.g. `nuget install BouncyCastle` (requires `nuget` https://www.nuget.org/)
+* Run `make hkdf` to verify and build the hkdf
+* Run tests using `lit test` (requires the LLVM Integrated Tester `pip install lit`)
